Loom/SpecMonad.lean
@@ -18,6 +18,39 @@ class LawfulMonadLift (w : outParam (Type u -> Type v)) [Monad m] [Monad w] [Mon
 
 export LawfulMonadLift (lift_pure lift_bind)
 
+class LawfulMonadLiftT (w : (Type u -> Type v)) [Monad m] [Monad w] [MonadLiftT m w] where
+  lift_pure {α : Type u} (x : α) : monadLift (pure (f := m) x) = pure (f := w) x
+  lift_bind {α : Type u} {β : Type u} (x : m α) (f : α -> m β) : monadLift (bind (m := m) x f) = bind (m := w) (monadLift x) (fun x => monadLift (f x))
+
+lemma lift_map {α : Type u} {β : Type u} (f : α -> β) (x : m α)
+  [Monad m] [Monad n] [LawfulMonad m] [LawfulMonad n] [MonadLiftT m n] [LawfulMonadLiftT m n] :
+  liftM (f <$> x) = f <$> liftM (n := n) x := by
+    rw [map_eq_pure_bind, liftM, LawfulMonadLiftT.lift_bind]
+    simp [LawfulMonadLiftT.lift_pure]
+
+instance [Monad m] : LawfulMonadLiftT m m where
+  lift_pure := by simp [monadLift, lift_pure]
+  lift_bind := by simp [monadLift, lift_bind]
+
+instance [Monad m] [LawfulMonad m] : LawfulMonadLiftT m (StateT σ m) where
+  lift_pure := by simp [monadLift, MonadLift.monadLift]; intros; ext; simp
+  lift_bind := by simp [monadLift, MonadLift.monadLift]; intros; ext; simp
+
+instance [Monad m] [LawfulMonad m] : LawfulMonadLiftT m (ReaderT σ m) where
+  lift_pure := by simp [monadLift, MonadLift.monadLift]; intros; ext; simp [ReaderT.run, pure, ReaderT.pure]
+  lift_bind := by simp [monadLift, MonadLift.monadLift]; intros; ext; simp [ReaderT.run, bind, ReaderT.bind]
+
+instance [Monad m] [LawfulMonad m] : LawfulMonadLiftT m (ExceptT ε m) where
+  lift_pure := by simp [monadLift, MonadLift.monadLift];
+  lift_bind := by simp [monadLift, MonadLift.monadLift]; intros; ext; simp
+
+instance [Monad m] [LawfulMonad m]
+  [Monad n] [LawfulMonad n] [MonadLiftT m n] [inst: LawfulMonadLiftT m n]
+  [Monad p] [LawfulMonad p] [MonadLift n p] [inst':LawfulMonadLift n p]
+  : LawfulMonadLiftT m p where
+    lift_pure := by simp [instMonadLiftTOfMonadLift, inst.lift_pure]; intros; apply inst'.lift_pure
+    lift_bind := by simp [instMonadLiftTOfMonadLift, inst.lift_bind]; intros; apply inst'.lift_bind
+
 alias EffectObservation := LawfulMonadLift
 
 -- class abbrev SpecMonad (m : Type u -> Type w) (w : Type u -> Type v) [Monad m] :=
